\documentclass{article}
\usepackage{amsmath}



\renewcommand{\vec}[1]{\mathbf{#1}}



\begin{document}

\section{One}

\begin{equation}
    a_{i}^k(n+1)=\sum_{j=1}^{2} w_{ij}^{k}o_{j}^{k}(n)+b_{i}^{k}-f_{i}^{k}(n), i=1,2; k=1,2,3,4
    \label{equ:1}
\end{equation}



\begin{equation}
    f_{i}^{k}(n)=\left\{
        \begin{array}{rcl}
            \gamma F^{k}(n) \cos(o_{i}^{k}(n)), i=1,\\
            \gamma F^{k}(n) \sin(o_{i}^{k}(n)), i=2,
        \end{array}
    \right.
    \label{equ:2}
\end{equation}



\begin{equation}
    o_{i}^{k}(n) = \tanh(a_{i}^{k}(n))
    \label{equ:3}
\end{equation}

\begin{equation}
    \sum_{k=1}^{4} F^{k}(n)=Mg
    \label{equ:4}
\end{equation}



\begin{equation}
    \vec{P}_{k}=(o_{1}^{k}(n),o_{2}^{k}(n))
    \label{<+label+>}
\end{equation}



%\begin{equation}
%   \vec{\vec{\phi}}= (acos(\frac{\vec{P}_{1} \vec{P}_{2}}{||\vec{P}_{1}|| ||\vec{P}_{2}||}), acos(\frac{\vec{P}_{1} \vec{P}_{3}}{||\vec{P}_{1}|| ||\vec{P}_{3}||}), acos(\frac{\vec{P}_{1} \vec{P}_{4}}{||\vec{P}_{1}|| ||\vec{P}_{4}||}))
%    \label{<+label+>}
%\end{equation}


\begin{equation}
    \vec{\vec{\phi}}= (\frac{\vec{P}_{1} \vec{P}_{2}}{||\vec{P}_{1}|| ||\vec{P}_{2}||}, \frac{\vec{P}_{1} \vec{P}_{3}}{||\vec{P}_{1}|| ||\vec{P}_{3}||}, \frac{\vec{P}_{1} \vec{P}_{4}}{||\vec{P}_{1}|| ||\vec{P}_{4}||})
    \label{<+label+>}
\end{equation}

%\begin{equation}
%    \dot{\vec{\phi}} = f(\vec{\phi})
%    \label{<+label+>}
%\end{equation}


From the initial condition:

$b_{i}^{k}=0.001$,

$o_{i}^{k}(0)=0.0$

The system will converge to the following result:

\begin{equation}
    \vec{\phi}=(0,0,1)
    \label{<+label+>}
\end{equation}




\section{TWO}


\begin{equation}
    a_{ik}(n+1)=\sum_{j=1}^{2} w_{ij}o_{jk}(n)+b_{ik}-f_{ik}(n), i=1,2; k=1,2,3,4 
    \label{<+label+>}
\end{equation}

\begin{equation}
    f_{ik}(n)=\left\{
        \begin{array}{rcl}
            \gamma F_{k3}(n) \cos(o_{ik}(n)), i=1,\\
            \gamma F_{k3}(n) \sin(o_{ik}(n)), i=2,
        \end{array}
    \right.
    \label{equ:2}
\end{equation}


\begin{equation}
    o_{ik}=\tanh(a_{ik})
    \label{<+label+>}
\end{equation}
\begin{equation}
\vec{o} = 
    \begin{pmatrix}
        o_{11} & o_{12} & o_{13} & o_{14} \\
        o_{21} & o_{22} & o_{23} & o_{24}
    \end{pmatrix}
    \label{<+label+>}
\end{equation}

\begin{equation}
    \mathbf{\vec{\theta}}=\Theta \vec{o} + \mathbf{\beta}
\end{equation}

\begin{equation}
    \vec{A}\vec{F}=\vec{b}
    \label{<+label+>}
\end{equation}

\begin{equation}
        \vec{A}=
        \begin{pmatrix}
            I_{3 \times 3} \dots I_{3 \times 3} \\
            \vec{P}_{1} \dots \vec{P}_{k}
        \end{pmatrix}
    \label{<+label+>}
\end{equation}


\begin{equation}
    \vec{F}=
    \begin{pmatrix}
        \vec{F}_{1} \dots \vec{F}_{k}
    \end{pmatrix}
    ^\top
    \label{<+label+>}
\end{equation}


\begin{equation}
    \vec{b}= 
    \begin{pmatrix}
        m(\ddot{\vec{P}_c} + \vec{g}) & \vec{I}_G \dot{\vec{\omega}}
    \end{pmatrix}
    ^\top
    \label{<+label+>}
\end{equation}



\end{document}
